remove unnecessary preconditions in load_save_regs_correct.v
(they follow from `program`, which checks that immediates
are within bounds, which is discharged at the very end via
translation validation)

use `stackalloc_words body` instead of
`stackalloc_size body / bytes_per_word`

wip in stackalloc proof, almost through function call

compiler/src/compiler/FlatToRiscvDef.v
@@ -203,9 +203,12 @@ Section FlatToRiscv1.
                    :: (load_regs regs (offset + bytes_per_word))
     end.
 
-  Fixpoint stackalloc_size(s: stmt Z): Z :=
+  (* number of words of stack allocation space needed *)
+  Fixpoint stackalloc_words(s: stmt Z): Z :=
     match s with
-    | SStackalloc x n body => Z.max 0 n + stackalloc_size body
+      (* ignore negative values, and round up values that are not divisible by bytes_per_word *)
+    | SStackalloc x n body => (Z.max 0 n + bytes_per_word - 1) / bytes_per_word
+                              + stackalloc_words body
     | _ => 0
     end.
 
@@ -289,20 +292,20 @@ Section FlatToRiscv1.
       (list Z * list Z * stmt Z) -> list Instruction :=
       fun '(argvars, resvars, body) =>
         let mod_vars := list_union Z.eqb (modVars_as_list Z.eqb body) argvars in
-        let scratchsize := stackalloc_size body in
-        let framesize := bytes_per_word * Z.of_nat (length argvars + length resvars + 1 + length mod_vars)
-                         + scratchsize in
+        let scratchwords := stackalloc_words body in
+        let framesize := bytes_per_word *
+                         (Z.of_nat (length argvars + length resvars + 1 + length mod_vars) + scratchwords) in
         [[ Addi sp sp (-framesize) ]] ++
         [[ compile_store access_size.word sp ra
-                         (scratchsize + bytes_per_word * (Z.of_nat (length mod_vars))) ]] ++
-        save_regs mod_vars scratchsize ++
-        load_regs argvars (scratchsize + bytes_per_word * (Z.of_nat (length mod_vars + 1 + length resvars))) ++
+                         (bytes_per_word * (Z.of_nat (length mod_vars) + scratchwords)) ]] ++
+        save_regs mod_vars (bytes_per_word * scratchwords) ++
+        load_regs argvars (bytes_per_word * (Z.of_nat (length mod_vars + 1 + length resvars) + scratchwords)) ++
         compile_stmt (mypos + 4 * (2 + Z.of_nat (length mod_vars + length argvars)))
-                     scratchsize body ++
-        save_regs resvars (scratchsize + bytes_per_word * (Z.of_nat (length mod_vars + 1))) ++
-        load_regs mod_vars scratchsize ++
+                     (bytes_per_word * scratchwords) body ++
+        save_regs resvars (bytes_per_word * (Z.of_nat (length mod_vars + 1) + scratchwords)) ++
+        load_regs mod_vars (bytes_per_word * scratchwords) ++
         [[ compile_load access_size.word ra sp
-                        (scratchsize + bytes_per_word * (Z.of_nat (length mod_vars))) ]] ++
+                        (bytes_per_word * (Z.of_nat (length mod_vars) + scratchwords)) ]] ++
         [[ Addi sp sp framesize ]] ++
         [[ Jalr zero ra 0 ]].
 
