compiler/src/compiler/FlatToRiscvFunctions.v
@@ -46,17 +46,20 @@ Section Proofs.
 
   Local Notation RiscvMachineL := MetricRiscvMachine.
 
-  Lemma stackalloc_size_nonneg: forall s,
-      0 <= stackalloc_size s.
+  Lemma stackalloc_words_nonneg: forall s,
+      0 <= stackalloc_words s.
   Proof.
-    induction s; simpl; blia.
+    assert (bytes_per_word = 4 \/ bytes_per_word = 8). {
+      unfold bytes_per_word. destruct width_cases as [E | E]; rewrite E; cbv; auto.
+    }
+    induction s; simpl; Z.div_mod_to_equations; blia.
   Qed.
 
   Lemma framesize_nonneg: forall argvars resvars body,
       0 <= framelength (argvars, resvars, body).
   Proof.
     intros. unfold framelength.
-    pose proof (stackalloc_size_nonneg body).
+    pose proof (stackalloc_words_nonneg body).
     assert (bytes_per_word = 4 \/ bytes_per_word = 8). {
       unfold bytes_per_word. destruct width_cases as [E | E]; rewrite E; cbv; auto.
     }
@@ -119,7 +122,7 @@ Section Proofs.
               | _ => fail 10000 P "is not a sep clause"
               end in
     lazymatch P with
-    | array ptsto_instr _ _ (compile_stmt _ _ ?Code) => Code
+    | array ptsto_instr _ _ (compile_stmt _ _ _ ?Code) => Code
     | ptsto_instr _ ?Instr => Instr
     | array ptsto_word _ _ ?Words => Words
     | functions _ _ ?E_Impl => E_Impl
@@ -149,7 +152,7 @@ Section Proofs.
     *)
     | |- @eq ?T _ _ => first [ unify T (list Instruction) | unify T (@env (@Semantics_params p)) ];
                        reflexivity
-    | H: fits_stack _ _ ?Code |- fits_stack _ _ ?Code => exact H
+    | H: fits_stack _ _ _ ?Code |- fits_stack _ _ _ ?Code => exact H
     | H: map.get ?R RegisterNames.sp = Some _ |- map.get ?R RegisterNames.sp = Some _ => exact H
     | |- ?G => assert_fails (has_evar G);
                solve [ simpl_addrs; solve_word_eq (@word_ok (@W (@def_params p)))
@@ -421,16 +424,11 @@ Section Proofs.
       assert (bytes_per_word = 4 \/ bytes_per_word = 8) as B48. {
         unfold bytes_per_word. destruct width_cases as [E | E]; rewrite E; cbv; auto.
       }
-      assert (0 <= stackalloc_size body / bytes_per_word) as ScratchNonneg. {
-        clear -B48.
-        pose proof (stackalloc_size_nonneg body) as P.
-        Z.div_mod_to_equations.
-        blia.
-      }
+      pose proof (stackalloc_words_nonneg body) as ScratchNonneg.
       assert (exists remaining_stack old_scratch old_modvarvals old_ra old_retvals old_argvals unused_scratch,
                  old_stackvals = remaining_stack ++ old_scratch ++ old_modvarvals ++ [old_ra] ++
                                                  old_retvals ++ old_argvals ++ unused_scratch /\
-                 List.length old_scratch = Z.to_nat (stackalloc_size body / bytes_per_word) /\
+                 List.length old_scratch = Z.to_nat (stackalloc_words body) /\
                  List.length old_modvarvals =
                     List.length (list_union Z.eqb (modVars_as_list Z.eqb body) argnames) /\
                  List.length old_retvals = List.length retnames /\
@@ -445,7 +443,7 @@ Section Proofs.
         split_from_right ToSplit ToSplit old_ras 1%nat.
         split_from_right ToSplit ToSplit old_modvarvals
                 (Datatypes.length (list_union Z.eqb (modVars_as_list Z.eqb body) argnames)).
-        split_from_right ToSplit ToSplit old_scratch (Z.to_nat (stackalloc_size body / bytes_per_word)).
+        split_from_right ToSplit ToSplit old_scratch (Z.to_nat (stackalloc_words body)).
         destruct old_ras as [|old_ra rest]; try discriminate.
         destruct rest; try discriminate.
         repeat match goal with
@@ -483,17 +481,6 @@ Section Proofs.
         - sidecondition.
         - sidecondition.
         - sidecondition.
-        - pose proof (NoDup_valid_FlatImp_vars_bound_length argnames) as A.
-          auto_specialize.
-          change (2 ^ 11) with 2048.
-          assert (bytes_per_word = 4 \/ bytes_per_word = 8) as B. {
-            clear. unfold bytes_per_word, Memory.bytes_per.
-            destruct width_cases.
-            + rewrite H. cbv. auto.
-            + rewrite H. cbv. auto.
-          }
-          replace (Datatypes.length argnames) with (Datatypes.length args) in A;
-            unfold Register, MachineInt in *; blia.
         - eapply map.getmany_of_list_extends; eassumption.
         - sidecondition.
         - unfold Register, MachineInt in *. blia.
@@ -603,7 +590,7 @@ Section Proofs.
       eauto.
     }
     eapply runsTo_trans. {
-      eapply save_regs_correct; simpl; cycle 2.
+      eapply save_regs_correct; simpl; cycle 1.
       2: rewrite map.get_put_same; reflexivity.
       1: exact P2.
       2: { eapply rearrange_footpr_subset; [ eassumption | wwcancel ]. }
@@ -617,20 +604,6 @@ Section Proofs.
       1: eassumption.
       2: reflexivity.
       1: wcancel_assumption.
-      pose proof (NoDup_valid_FlatImp_vars_bound_length (list_union Z.eqb (modVars_as_list Z.eqb body) argnames)) as A.
-      specialize_hyp A.
-      - eapply list_union_preserves_NoDup. assumption.
-      - apply union_Forall.
-        * apply modVars_as_list_valid_FlatImp_var. assumption.
-        * assumption.
-      - change (2 ^ 11) with 2048.
-        assert (bytes_per_word = 4 \/ bytes_per_word = 8) as B. {
-          clear. unfold bytes_per_word, Memory.bytes_per.
-          destruct width_cases.
-          + rewrite H. cbv. auto.
-          + rewrite H. cbv. auto.
-        }
-        clear -A B. unfold Register, MachineInt in *. blia.
     }
 
     simpl.
@@ -646,7 +619,7 @@ Section Proofs.
     eapply runsTo_trans. {
       eapply load_regs_correct with
           (vars := argnames) (values := argvs);
-        simpl; cycle 2.
+        simpl; cycle 1.
       - rewrite map.get_put_same. reflexivity.
       - assumption.
       - eapply rearrange_footpr_subset; [eassumption|wwcancel].
@@ -654,30 +627,6 @@ Section Proofs.
       - reflexivity.
       - assumption.
       - assumption.
-      - pose proof (NoDup_valid_FlatImp_vars_bound_length retnames) as A.
-        pose proof (NoDup_valid_FlatImp_vars_bound_length argnames) as A'.
-        auto_specialize.
-        change (2 ^ 11) with 2048.
-        assert (bytes_per_word = 4 \/ bytes_per_word = 8) as B. {
-          clear. unfold bytes_per_word, Memory.bytes_per.
-          destruct width_cases.
-          + rewrite H. cbv. auto.
-          + rewrite H. cbv. auto.
-        }
-        pose proof (NoDup_valid_FlatImp_vars_bound_length (list_union Z.eqb (modVars_as_list Z.eqb body) argnames)) as A''.
-        specialize_hyp A''.
-        + apply list_union_preserves_NoDup. assumption.
-        + apply union_Forall.
-          * apply modVars_as_list_valid_FlatImp_var. assumption.
-          * assumption.
-        + clear -A A' A'' B.
-          change BinIntDef.Z.eqb with Z.eqb.
-          unfold Register, MachineInt in *.
-          match type of A'' with
-          | (?x <= _)%nat => forget x as L
-          end.
-          destruct B as [B | B]; rewrite B; (* <-- TODO once we're on 8.10 delete this line *)
-            blia.
     }
 
     simpl.
@@ -688,15 +637,28 @@ Section Proofs.
            | m: _ |- _ => destruct_RiscvMachine m
            end.
     subst.
+    match goal with
+    | H: fits_stack _ ?x _ _ |- _ => revert H; simpl_addrs; intro FS
+    end.
+    match type of FS with
+    | _ _ ?x _ _ => ring_simplify x in FS
+    end.
 
     (* execute function body *)
     eapply runsTo_trans. {
-      unfold good_reduced_e_impl, good_e_impl, valid_FlatImp_fun in *. simp.
+      unfold good_e_impl, valid_FlatImp_fun in *. simp.
       eapply IHexec with (g := {|
         p_sp := word.sub p_sp !(bytes_per_word * FL);
         e_pos := e_pos;
-        program_base := program_base; |});
-      after_IH;
+        e_impl := map.remove e_impl fname;
+        program_base := program_base;
+      |});
+      simpl_MetricRiscvMachine_get_set;
+      simpl_g_get;
+      rewrite ?@length_save_regs, ?@length_load_regs in *;
+      unfold Register, MachineInt in *;
+      simpl_word_exprs (@word_ok (@W (@def_params p)));
+      ssplit;
       subst FL.
       all: try safe_sidecond.
       all: try safe_sidecond.
@@ -749,6 +711,19 @@ Section Proofs.
         eapply preserve_regs_initialized_after_put.
         assumption.
       }
+      {
+        exists (remaining_stack ++ old_scratch). split.
+        - simpl_addrs. blia.
+        - wcancel_assumption.
+      }
+      {
+        match goal with
+        | H:valid_machine {| getMachine := _; getMetrics := ?M |}
+          |- valid_machine {| getMachine := _; getMetrics := ?M |} => eqexact H
+        end.
+        simpl_addrs.
+        reflexivity.
+      }
     }
 
     simpl.
@@ -772,7 +747,7 @@ Section Proofs.
 
     (* save results onto stack *)
     eapply runsTo_trans. {
-      eapply save_regs_correct with (vars := retnames); simpl; cycle 2.
+      eapply save_regs_correct with (vars := retnames); simpl; cycle 1.
       - eapply map.getmany_of_list_extends; try eassumption.
       - eassumption.
       - instantiate (1 := old_retvals). unfold Register, MachineInt in *. blia.
@@ -783,29 +758,6 @@ Section Proofs.
       - eapply Forall_impl; cycle 1.
         + eassumption.
         + apply valid_FlatImp_var_implies_valid_register.
-      - pose proof (NoDup_valid_FlatImp_vars_bound_length retnames) as A.
-        auto_specialize.
-        change (2 ^ 11) with 2048.
-        assert (bytes_per_word = 4 \/ bytes_per_word = 8) as B. {
-          clear. unfold bytes_per_word, Memory.bytes_per.
-          destruct width_cases.
-          + rewrite H. cbv. auto.
-          + rewrite H. cbv. auto.
-        }
-        pose proof (NoDup_valid_FlatImp_vars_bound_length (list_union Z.eqb (modVars_as_list Z.eqb body) argnames)) as A''.
-        specialize_hyp A''.
-        + apply list_union_preserves_NoDup. assumption.
-        + apply union_Forall.
-          * apply modVars_as_list_valid_FlatImp_var. assumption.
-          * assumption.
-        + clear -A A'' B.
-          change BinIntDef.Z.eqb with Z.eqb.
-          unfold Register, MachineInt in *.
-          match type of A'' with
-          | (?x <= _)%nat => forget x as L
-          end.
-          destruct B as [B | B]; rewrite B; (* <-- TODO once we're on 8.10 delete this line *)
-            blia.
     }
 
     simpl.
@@ -821,7 +773,7 @@ Section Proofs.
     eapply runsTo_trans. {
       eapply load_regs_correct with
           (vars := (list_union Z.eqb (modVars_as_list _ body) argnames)) (values := newvalues);
-        simpl; cycle 2.
+        simpl; cycle 1.
       - eassumption.
       - repeat match goal with
                | H: map.getmany_of_list _ _ = Some _ |- _ =>
@@ -837,22 +789,6 @@ Section Proofs.
       - apply union_Forall.
         + apply modVars_as_list_valid_FlatImp_var. assumption.
         + assumption.
-      - pose proof (NoDup_valid_FlatImp_vars_bound_length (list_union Z.eqb (modVars_as_list Z.eqb body) argnames)) as A.
-        specialize_hyp A.
-        + apply list_union_preserves_NoDup. assumption.
-        + apply union_Forall.
-          * apply modVars_as_list_valid_FlatImp_var. assumption.
-          * assumption.
-        + change (2 ^ 11) with 2048.
-          assert (bytes_per_word = 4 \/ bytes_per_word = 8) as B. {
-            clear. unfold bytes_per_word, Memory.bytes_per.
-            destruct width_cases.
-            - rewrite H. cbv. auto.
-            - rewrite H. cbv. auto.
-          }
-          clear -A B.
-          destruct B as [B | B]; rewrite B; (* <-- TODO once we're on 8.10 delete this line *)
-            blia.
     }
 
     simpl.
@@ -1002,32 +938,6 @@ Section Proofs.
         cbn [seps].
         wcancel.
       - reflexivity.
-      - pose proof (NoDup_valid_FlatImp_vars_bound_length argnames) as A.
-        pose proof (NoDup_valid_FlatImp_vars_bound_length retnames) as A'.
-        auto_specialize.
-        change (2 ^ 11) with 2048.
-        assert (bytes_per_word = 4 \/ bytes_per_word = 8) as B. {
-          clear. unfold bytes_per_word, Memory.bytes_per.
-          destruct width_cases.
-          + rewrite H. cbv. auto.
-          + rewrite H. cbv. auto.
-        }
-        unfold Register, MachineInt in *.
-        replace (Datatypes.length argnames) with (Datatypes.length args) in A by blia.
-        match goal with
-        | H: map.getmany_of_list _ retnames = Some _ |- _ =>
-          rename H into G; move G at bottom
-        end.
-        apply map.getmany_of_list_length in G.
-        match goal with
-        | H: map.putmany_of_list_zip _ retvs _ = Some _ |- _ =>
-          rename H into G'; move G' at bottom
-        end.
-        apply map.putmany_of_list_zip_sameLength in G'.
-        replace (Datatypes.length retnames) with (Datatypes.length binds) in A' by blia.
-        clear -A A' B.
-        destruct B as [B | B]; rewrite B; (* <-- TODO once we're on 8.10 delete this line *)
-          blia.
       - subst FL.
         simpl_addrs.
         rewrite map.get_put_same. f_equal. solve_word_eq word_ok.
@@ -1480,7 +1390,7 @@ Section Proofs.
       (* PARAMRECORDS *)
       change Z with Register in *.
       subst FL new_ra. simpl_addrs.
-      split. { ring. (* faster than lia *) }
+      split. 2: {
       use_sep_assumption.
       wseplog_pre.
       pose proof functions_expose as P.
@@ -1505,6 +1415,28 @@ Section Proofs.
              end.
       rewrite! length_save_regs. rewrite! length_load_regs. (* <- needs to be before simpl_addrs *)
       simpl_addrs. simpl. (* PARAMRECORDS *)
+
+      assert (
+(array scalar !bytes_per_word
+                   (p_sp -
+                    !(bytes_per_word *
+                      (stackalloc_words body +
+                       (#(Datatypes.length argnames) + #(Datatypes.length binds) + 1 +
+                        #(Datatypes.length newvalues)))) -
+                    !(bytes_per_word * (#(Datatypes.length stack_trash) - stackalloc_words body))) stack_trash)
+=
+(array scalar !bytes_per_word
+   (p_sp -
+    !(bytes_per_word *
+      (#(Datatypes.length stack_trash) - stackalloc_words body +
+       (stackalloc_words body +
+        (#(Datatypes.length newvalues) +
+         (#(Datatypes.length binds) + (#(Datatypes.length argnames) + rem_framewords) + 1))) - rem_framewords)))
+   remaining_stack)).
+      {
+        f_equal.
+
+
       wcancel.
     + reflexivity.
     + assumption.
